WIP cbor_map_sort

share/steel/examples/pulse/dice/cbor/CBOR.Spec.Map.fst
@@ -76,3 +76,125 @@ let rec list_sorted_map_entry_order_no_repeats
     list_sorted_map_entry_order_no_repeats key_order q;
     list_sorted_map_entry_order_not_memP_tail key_order a q
 
+let rec list_tot_for_all_order_trans
+    (#t1: Type)
+    (order: t1 -> t1 -> bool {
+      (forall x . order x x == false) /\
+      (forall x y z . (order x y /\ order y z) ==> order x z)
+    })
+    (k1v1: _)
+    (k2v2: _)
+    (l1: list t1)
+  : Lemma
+  (requires (order k1v1 k2v2 /\
+    List.Tot.for_all (order k2v2) l1
+  ))
+  (ensures (
+    List.Tot.for_all (order k1v1) l1
+  ))
+  (decreases l1)
+= match l1 with
+  | [] -> ()
+  | _ :: q -> list_tot_for_all_order_trans order k1v1 k2v2 q
+
+let rec list_ghost_assoc
+  (#key: Type)
+  (#value: Type)
+  (k: key)
+  (m: list (key & value))
+: GTot (option value)
+  (decreases m)
+= match m with
+  | [] -> None
+  | (k', v') :: m' ->
+    if FStar.StrongExcludedMiddle.strong_excluded_middle (k == k')
+    then Some v'
+    else list_ghost_assoc k m'
+
+let rec list_ghost_assoc_append
+    (#tk #tv: Type)
+    (k: tk)
+    (l1 l2: list (tk & tv))
+: Lemma
+    (ensures (list_ghost_assoc k (l1 `List.Tot.append` l2) == (
+        match list_ghost_assoc k l1 with
+        | Some v -> Some v
+        | None -> list_ghost_assoc k l2
+    )))
+    (decreases l1)
+= match l1 with
+| [] -> ()
+| (k1, _ ) :: q1 ->
+    if FStar.StrongExcludedMiddle.strong_excluded_middle (k == k1)
+    then ()
+    else list_ghost_assoc_append k q1 l2
+
+[@@noextract_to "krml"] noextract
+let rec map_sort_merge
+  (#t1 #t2: Type)
+  (key_compare: t1 -> t1 -> int)
+  (accu: list (t1 & t2))
+  (l1: list (t1 & t2))
+  (l2: list (t1 & t2))
+: Tot (bool & list (t1 & t2))
+  (decreases (List.Tot.length l1 + List.Tot.length l2))
+= match l1, l2 with
+  |  (k1, v1) :: l1', (k2, v2) :: l2' ->
+    begin let c = key_compare k1 k2 in
+      if c = 0
+      then (false, accu `List.Tot.append` (l1 `List.Tot.append` l2))
+      else if c < 0
+      then map_sort_merge key_compare (accu `List.Tot.append` [(k1, v1)]) l1' l2
+      else map_sort_merge key_compare (accu `List.Tot.append` [(k2, v2)]) l1' ((k1, v1) :: l2') // this is not a stable sort
+    end
+  | [], _ -> (true, accu `List.Tot.append` l2)
+  | _, [] -> (true, accu `List.Tot.append` l1)
+
+let rec list_splitAt_length
+  (#t: Type)
+  (n: nat)
+  (l: list t)
+: Lemma
+  (requires (List.Tot.length l >= n))
+  (ensures (
+    let (l1, l2) = List.Tot.splitAt n l in
+    List.Tot.length l1 == n /\
+    List.Tot.length l1 + List.Tot.length l2 == List.Tot.length l
+  ))
+  [SMTPat (List.Tot.splitAt n l)]
+= if n = 0 then () else list_splitAt_length (n - 1) (List.Tot.tl l)
+
+[@@noextract_to "krml"] noextract
+let rec map_sort
+  (#t1 #t2: Type)
+  (key_compare: t1 -> t1 -> int)
+  (l: list (t1 & t2))
+: Tot (bool & list (t1 & t2))
+  (decreases (List.Tot.length l))
+= let len = List.Tot.length l in
+  if len < 2
+  then (true, l)
+  else
+    let (l1, l2) = List.Tot.splitAt (len / 2) l in
+    let (res, l1') = map_sort key_compare l1 in
+    if not res
+    then (false, l1' `List.Tot.append` l2)
+    else
+      let (res, l2') = map_sort key_compare l2 in
+      if not res
+      then (false, l1' `List.Tot.append` l2')
+      else map_sort_merge key_compare [] l1' l2'
+
+let map_sort_correct
+  (#t1 #t2: Type)
+  (key_order: t1 -> t1 -> bool)
+  (key_compare: t1 -> t1 -> int)
+  (l: list (t1 & t2))
+: Lemma
+  (let (res, l') = map_sort key_compare l in
+    (forall pre suff . List.Tot.no_repeats_p (pre `List.Tot.append` (List.Tot.map fst l' `List.Tot.append` suff)) <==> List.Tot.no_repeats_p (pre `List.Tot.append` (List.Tot.map fst l `List.Tot.append` suff))) /\
+    (if res
+    then (List.Tot.sorted (map_entry_order key_order _) l' /\ (forall k . list_ghost_assoc k l' == list_ghost_assoc k l))
+    else ~ (List.Tot.no_repeats_p (List.Tot.map fst l)))
+  )
+= admit ()
